Define heaplang interpreter and prove soundness.

src/heaplang/adequacy.v
@@ -5,41 +5,41 @@ From iris.itree Require Import wpi ub itree choice state later handler void.
 From iris.itree.threadpool Require Import ctrace handler interleaving.
 From iris.itree.heaplang Require Import lang.
 
-Definition heaplang_irel {R} (t : itree heaplangE R) (σ : state) (n : option nat)
-  (te : itree voidE (option ((state * (R + last_thread_killed)) + later_exhausted))) : Prop :=
+Definition heaplang_irel {R} (σ : state) (n : option nat) (t : itree heaplangE R)
+  (te : itree voidE ((state * (R + last_thread_killed)) + later_exhausted + ub_crash)) : Prop :=
   ∃ t1 t2 t3,
     threadpool_irel t t1 ∧
     demonic_irel t1 t2 ∧
     state_irel σ t2 t3 ∧
-    te ≈ ub_ifn (insert_voidE (later_ifn n t3)).
+    te = ub_ifn (insert_voidE (later_ifn n t3)).
 
 Definition heaplang_eval (e : expr) (σ : state) (n : option nat)
   (* TODO: Can remove the itree here? How would we represent diverging
   programs when not using later? *)
-  (exec: itree voidE (option ((state * (val + last_thread_killed)) + later_exhausted))) : Prop :=
-  heaplang_irel (v ← compile_expr e ; yield_if_not_val e ;; Ret v) σ n exec.
+  (exec: itree voidE ((state * (val + last_thread_killed)) + later_exhausted + ub_crash)) : Prop :=
+  heaplang_irel σ n (v ← compile_expr e ; yield_if_not_val e ;; Ret v) exec.
 
 Section adequacy.
   Context {Σ} `{!invGS Σ} `{!heaplangHGS Σ}.
 
   Lemma heaplang_adequacy_irel R t σ te (Φ : R → iProp Σ) n lat :
-    heaplang_irel t σ n te →
-    (lat = Later ↔ is_Some n) →
+    heaplang_irel σ n t te →
+    (lat = Later → is_Some n) →
     state_interp σ -∗
     £ (default 0 n) -∗
     WPi t @ heaplangH lat; ⊤ {{ Φ }} -∗
     |={⊤, ∅}=> ∃ v, ⌜te ≈ Ret v⌝ ∗
       match v with
-      | None => False
-      | Some (inr LaterExhausted) => ⌜lat = Later⌝
-      | Some (inl σr) => |={∅, ⊤}=> let (σ, r) := σr in state_interp σ ∗
+      | inr UbCrash => False
+      | inl (inr LaterExhausted) => ⌜is_Some n⌝
+      | inl (inl σr) => |={∅, ⊤}=> let (σ, r) := σr in state_interp σ ∗
           match r with | inl v => Φ v | inr _ => True end
       end.
   Proof.
     iIntros ((?&?&?&?&?&?&Hte) ?) "Hs Hlc Hwp".
     iDestruct (threadpool_adequacy with "Hwp") as "Hwp"; [done|].
-    iDestruct (demonicH_adequate with "Hwp") as "Hwp"; [done|].
-    iDestruct (wpi_state with "Hs Hwp") as "Hwp"; [done|].
+    iDestruct (demonic_adequacy with "Hwp") as "Hwp"; [done|].
+    iDestruct (state_adequacy with "Hs Hwp") as "Hwp"; [done|].
     rewrite -wpi_clear_mask. iMod "Hwp".
     iDestruct (later_adequacy_empty with "Hwp Hlc") as "Hwp"; [done|].
     iDestruct (voidE_adequacy with "Hwp") as "Hwp".
@@ -50,16 +50,16 @@ Section adequacy.
 
   Lemma heaplang_adequacy_eval e σ te (Φ : val → iProp Σ) n lat :
     heaplang_eval e σ n te →
-    (lat = Later ↔ is_Some n) →
+    (lat = Later → is_Some n) →
     state_interp σ -∗
     £ (default 0 n) -∗
     heap_inv -∗
     WP e @ lat; ⊤ {{ Φ }} -∗
     |={⊤, ∅}=> ∃ v, ⌜te ≈ Ret v⌝ ∗
       match v with
-      | None => False
-      | Some (inr LaterExhausted) => ⌜lat = Later⌝
-      | Some (inl σr) => |={∅, ⊤}=> let (σ, r) := σr in state_interp σ ∗
+      | inr UbCrash => False
+      | inl (inr LaterExhausted) => ⌜is_Some n⌝
+      | inl (inl σr) => |={∅, ⊤}=> let (σ, r) := σr in state_interp σ ∗
           match r with | inl v => Φ v | inr _ => True end
       end.
   Proof.
