src/heaplang/interpreter.v
@@ -1,0 +1,82 @@
+From ITree Require Import ITree Eqit.
+From iris Require Import invariants ghost_map.
+From iris.proofmode Require Import proofmode.
+From iris.itree Require Import wpi ub itree choice state later handler void interpreter.
+From iris.itree.threadpool Require Import handler interleaving scheduler.
+From iris.itree.heaplang Require Import lang adequacy.
+
+Definition heaplang_ifn {R} (σ : state) (n : option nat) (t : itree heaplangE R) :
+  itree voidE ((state * (R + last_thread_killed)) + later_exhausted + ub_crash) :=
+  ub_ifn (insert_voidE (later_ifn n (state_ifn σ (demonic_ifn (threadpool_ifn t))))).
+
+Lemma heaplang_ifn_irel {R} (t : itree heaplangE R) (σ : state) (n : option nat) :
+  heaplang_irel σ n t (heaplang_ifn σ n t).
+Proof.
+  eexists. eexists. eexists.
+  split; first apply threadpool_ifn_irel.
+  split; first apply demonic_ifn_irel.
+  split; first apply state_ifn_irel.
+  reflexivity.
+Qed.
+
+Variant timeout := Timeout.
+
+Definition heaplang_eval_itree σ n e :=
+  heaplang_ifn σ (Some n) (v ← compile_expr e ; yield_if_not_val e ;; Ret v).
+
+Definition heaplang_interpreter σ (n : nat) (e : expr) : (state * (val + last_thread_killed)) + ub_crash + timeout :=
+  match exec n (heaplang_eval_itree σ n e) with
+  | None => inr Timeout
+  | Some (inl (inr LaterExhausted)) => inr Timeout
+  | Some (inl (inl r)) => inl (inl r)
+  | Some (inr UbCrash) => inl (inr UbCrash)
+  end.
+
+Lemma heaplang_interpreter_adequacy `{!invGS Σ} `{!heaplangHGS Σ} m e σ n Φ :
+  state_interp σ -∗
+  £ n -∗
+  heap_inv -∗
+  WP e @ m; ⊤ {{ Φ }} -∗
+  |={⊤, ∅}=>
+    match heaplang_interpreter σ n e with
+    | inr Timeout => True
+    | inl (inr UbCrash) => False
+    | inl (inl (σ, r)) => state_interp σ ∗
+        match r with | inl v => Φ v | inr LastThreadKilled => True end
+    end.
+Proof.
+  iIntros "Hstate Hlc Hinv Hwp".
+  iDestruct (heaplang_adequacy_eval e σ (heaplang_eval_itree σ n e) with "Hstate [Hlc] Hinv Hwp") as "Heval".
+  { apply heaplang_ifn_irel. }
+  { eauto. }
+  { done. }
+  iMod "Heval" as "[%v [%Heval HΦ]]".
+  rewrite /heaplang_interpreter. destruct (exec n (heaplang_eval_itree σ n e)) eqn:Heq.
+  * apply exec_eutt with (t' := (Ret v)) in Heq as [n' Heq]; last done.
+    destruct n'; first done. injection Heq as <-.
+    destruct v.
+    + destruct s.
+      -- iMod "HΦ". destruct p as [σ0 [v|[]]]; iApply fupd_mask_intro; eauto.
+      -- by destruct l.
+    + by destruct u.
+  * destruct v; eauto.
+Qed.
+
+Lemma heaplang_interpreter_soundness `{!invGpreS Σ} `{!heaplangHGpreS Σ} m e σ n φ :
+  (∀ `{!invGS Σ} `{!heaplangHGS Σ}, ⊢ WP e @ m; ⊤ {{ v, ⌜φ v⌝ }}) →
+  match heaplang_interpreter σ n e with
+  | inr Timeout => True
+  | inl (inr UbCrash) => False
+  | inl (inl (_, inl v)) => φ v
+  | inl (inl (_, inr LastThreadKilled)) => True
+  end.
+Proof.
+  intros Hwp. apply: (heaplang_soundness n).
+  iIntros (? ?) "#Hinv Hstate Hlc".
+  iDestruct Hwp as "Hwp".
+  iDestruct (heaplang_interpreter_adequacy m e σ n with "Hstate Hlc Hinv Hwp") as "Hφ".
+  iMod "Hφ". iModIntro.
+  iApply step_fupdN_intro; first done. iModIntro.
+  destruct (heaplang_interpreter σ n e) as [[[σ' [v|[]]]|[]]|[]]; eauto.
+  iDestruct "Hφ" as "[_ $]".
+Qed.
